Program initialization is now using normal memory load requests

Kami/Ex/ProcFDCorrect.v
@@ -28,7 +28,7 @@ Section FetchDecode.
             (getDst: DstT instBytes rfIdx)
             (exec: ExecT iaddrSize instBytes dataBytes)
             (getNextPc: NextPcT iaddrSize instBytes dataBytes rfIdx)
-            (alignAddr: AlignAddrT addrSize)
+            (alignInst: AlignInstT instBytes dataBytes)
             (predictNextPc: forall ty, fullType ty (SyntaxKind (Pc iaddrSize)) -> (* pc *)
                                        Expr ty (SyntaxKind (Pc iaddrSize))).
 
@@ -82,13 +82,14 @@ Section FetchDecode.
   Definition fetchDecode := fetchDecode
                               getOptype getLdDst getLdAddr getLdSrc calcLdAddr
                               getStAddr getStSrc calcStAddr getStVSrc
-                              getSrc1 getSrc2 getDst predictNextPc d2ePack
+                              getSrc1 getSrc2 getDst alignInst predictNextPc d2ePack
                               f2dPack f2dRawInst f2dCurPc f2dNextPc f2dEpoch
                               pcInit.
   Definition fetchNDecode := ProcThreeStage.fetchDecode
+                               "rqFromProc"%string "rsToProc"%string
                                getOptype getLdDst getLdAddr getLdSrc calcLdAddr
                                getStAddr getStSrc calcStAddr getStVSrc
-                               getSrc1 getSrc2 getDst d2ePack predictNextPc
+                               getSrc1 getSrc2 getDst alignInst d2ePack predictNextPc
                                pcInit.
 
   Hint Unfold fetchDecode: ModuleDefs. (* for kinline_compute *)
@@ -120,7 +121,7 @@ Section FetchDecode.
   Definition fetchDecodeInl := ProcFDInl.fetchDecodeInl
                                  getOptype getLdDst getLdAddr getLdSrc calcLdAddr
                                  getStAddr getStSrc calcStAddr getStVSrc
-                                 getSrc1 getSrc2 getDst predictNextPc d2ePack
+                                 getSrc1 getSrc2 getDst alignInst predictNextPc d2ePack
                                  f2dPack f2dRawInst f2dCurPc f2dNextPc f2dEpoch
                                  pcInit.
 
