Kami/Ex/ProcThreeStInl.v
@@ -22,7 +22,7 @@ Section Inlined.
             (getDst: DstT instBytes rfIdx)
             (exec: ExecT iaddrSize instBytes dataBytes)
             (getNextPc: NextPcT iaddrSize instBytes dataBytes rfIdx)
-            (alignAddr: AlignAddrT addrSize)
+            (alignInst: AlignInstT instBytes dataBytes)
             (predictNextPc: forall ty, fullType ty (SyntaxKind (Pc iaddrSize)) -> (* pc *)
                                        Expr ty (SyntaxKind (Pc iaddrSize))).
 
@@ -73,7 +73,7 @@ Section Inlined.
 
   Definition p3st := p3st getOptype getLdDst getLdAddr getLdSrc calcLdAddr
                           getStAddr getStSrc calcStAddr getStVSrc
-                          getSrc1 getSrc2 getDst exec getNextPc alignAddr predictNextPc
+                          getSrc1 getSrc2 getDst exec getNextPc alignInst predictNextPc
                           d2ePack d2eOpType d2eDst d2eAddr d2eVal1 d2eVal2
                           d2eRawInst d2eCurPc d2eNextPc d2eEpoch
                           e2wPack e2wDecInst e2wVal init.
@@ -85,7 +85,7 @@ Section Inlined.
                   (procThreeStage_ModEquiv getOptype getLdDst getLdAddr getLdSrc calcLdAddr
                                            getStAddr getStSrc calcStAddr getStVSrc
                                            getSrc1 getSrc2 getDst exec
-                                           getNextPc alignPc alignAddr predictNextPc
+                                           getNextPc alignPc alignInst predictNextPc
                                            d2ePack d2eOpType d2eDst d2eAddr d2eVal1 d2eVal2
                                            d2eRawInst d2eCurPc d2eNextPc d2eEpoch
                                            e2wPack e2wDecInst e2wVal init
