Kami/Ex/ProcThreeStInv.v
@@ -27,7 +27,7 @@ Section Invariants.
             (getDst: DstT instBytes rfIdx)
             (exec: ExecT iaddrSize instBytes dataBytes)
             (getNextPc: NextPcT iaddrSize instBytes dataBytes rfIdx)
-            (alignAddr: AlignAddrT addrSize)
+            (alignInst: AlignInstT instBytes dataBytes)
             (predictNextPc: forall ty, fullType ty (SyntaxKind (Pc iaddrSize)) -> (* pc *)
                                        Expr ty (SyntaxKind (Pc iaddrSize))).
 
@@ -105,7 +105,7 @@ Section Invariants.
   Definition p3stInl := projT1 (p3stInl getOptype getLdDst getLdAddr getLdSrc calcLdAddr
                                         getStAddr getStSrc calcStAddr getStVSrc
                                         getSrc1 getSrc2 getDst exec getNextPc
-                                        alignAddr predictNextPc
+                                        alignInst predictNextPc
                                         d2ePack d2eOpType d2eDst d2eAddr d2eVal1 d2eVal2
                                         d2eRawInst d2eCurPc d2eNextPc d2eEpoch
                                         e2wPack e2wDecInst e2wVal init).
